save before major restructure

Disjoint.v
@@ -12,66 +12,69 @@ Require Evaluation Util.
 Module Disjoint.
   Import Evaluation.Evaluation Util.
 
-  Parameter branch: Lab -> option (Lab * Lab * Var * Var).
+  Parameter branch: Lab -> list Var.
 
-  Definition is_branch br x := exists tt ff xb, branch br = Some (tt, ff, x, xb).
+  Definition is_branch br x := x ∈ branch br.
 
   Parameter val_true : Val -> bool.
 
   Parameter branch_spec :
-    forall b, match branch b with
-              | Some (t, f, x, xb) => t =/= f /\
-                                      forall i s k, eff (b, i, s) = Some k ->
-                                                    lab_of k = (if val_true (s x) then t else f)
-              | None => forall i i' s s' k k', eff (b, i, s) = Some k ->
-                                               eff (b, i', s') = Some k' ->
-                                               lab_of k = lab_of k'
-              end.
+    forall b, exists (d : list Var -> Lab), forall s, match (eff' (b, s)) with
+                                      | Some (q,_) => q = d (branch b)
+                                      | None => True
+                                      end.
 
-  Parameter branch_spec_var : 
-    forall b t f x xb, branch b = Some (t, f, x, xb) -> is_def xb b t = true /\ is_def xb b f = true /\
-                                                        forall b', b =/= b' -> forall p, is_def xb b' p = false.
+(*  Parameter in_out_spec :
+    forall p q q', (exists x, is_branch p x) -> q --> p -> q' --> p -> q = q'.*)
 
-  Parameter in_out_spec :
-    forall p q q', (exists x, is_branch p x) -> q --> p -> q' --> p -> q = q'.
-
-  Definition DisjointBranch (s : Lab) (x : Var) (qt qf : Lab) (π ϕ : list Lab) :=
-    CPath s qt (nl_rcons π s) /\ CPath s qf (nl_rcons ϕ s) /\ is_branch s x /\ Disjoint π ϕ.
-
-  Parameter splits : Lab -> list (Lab * Var).
-
-  Parameter splits_spec : forall conv br x,
-      (exists qt qf π ϕ, qt --> conv /\ qf --> conv /\ qt =/= qf /\
-                    DisjointBranch br x qt qf π ϕ) <->
-      List.In (br, x) (splits conv).
-
-  Parameter loop_splits : Lab -> list (Lab * Var).
-
-  Parameter loop_splits_spec : forall p br x,
-      (exists qh π ϕ, in_loop br qh /\ qh <> p /\ DisjointBranch br x qh p π ϕ)
-      <-> In (br, x) (loop_splits p).
-
-  Lemma split_last_common s x p l1 l2 :
-    Path root p (p :<: l1)
-    -> Path root p (p :<: l2)
-    -> In (s,x) (splits p)
-    -> last_common l1 l2 s.
-  Admitted.
   
-  Lemma last_common_split s x p l1 l2 :
+  Definition DisjointBranch (s : Lab) (xl : list Var) (qt qf : Lab) (π ϕ : list Lab) :=
+    CPath s qt (π >: s) /\ CPath s qf (ϕ >: s) /\ branch s =' xl /\ Disjoint π ϕ.
+
+  Parameter path_splits : Lab -> list (Lab * Lab * Lab * list Var).
+
+  Parameter loop_splits : Lab -> Lab -> list (Lab * Lab * Lab * list Var).
+
+  Definition pl_split `{Graph Lab} (qh qe q1 q2 br : Lab) (xl : list Var) :=
+      (exists π ϕ, Path br qh (π >: q1 :>: br)
+              /\ Path br qe (ϕ >: q2 :>: br)
+              /\ Disjoint (tl π :r: q1) (tl ϕ :r: q2)
+              /\ branch br =' xl).
+
+  Set Printing All.
+
+  Parameter path_splits_spec : forall `{Graph Lab} p q1 q2 br xl,
+      pl_split p p q1 q2 br xl <->
+      (br, q1, q2, xl) ∈ path_splits p.
+  
+  Parameter loop_splits_spec : forall `{Graph Lab} qh qe q1 q2 br xl,
+      in_loop br qh /\ (* otherwise some splits would be considered as loop splits *)
+      pl_split qh qe q1 q2 br xl <->
+      (br, q1, q2, xl) ∈ loop_splits qh qe.
+  
+(*  Parameter preceding_loops : Lab -> Lab -> list (Lab * Lab).
+
+  Parameter preceding_loops_spec : forall s p qh qe, (qh, qe) ∈ preceding_loops p s
+                                              <-> loop_head qh
+                                                /\ qh ∈ loop_exit qe
+                                                /\ in_loop s qh
+                                                /\ ~ in_loop p qh
+                                                /\ qe --> p.*)
+  
+  Lemma last_common_split s x p q1 q2 l1 l2 :
     Path root p (p :<: l1)
     -> Path root p (p :<: l2)
     -> last_common l1 l2 s
-    -> In (s,x) (splits p).
+    -> In (s,q1,q2,x) (path_splits p).
   Admitted.
   
-  Lemma last_common_split_loopsplit s x s' l1 l2 k :
+(*  Lemma last_common_split_loopsplit s x s' l1 l2 k :
     Tr (k :<: l1)
     -> Tr (k :<: l2)
     -> In (s,x) (splits (lab_of k))
     -> last_common (ne_map fst l1) (ne_map fst l2) s'
     -> In (fst s') (map fst (loop_splits s)).
-  Admitted.
+  Admitted.*)
   
   Lemma disjoint_map_fst {A B : Type} (l1 l2 : list (A*B)) (l1' l2' : list A) :
     l1' = map fst l1
@@ -81,7 +84,7 @@ Module Disjoint.
   Admitted.
 
   Definition innermost_loop p qh :=
-    in_loop p qh /\ forall qh', in_loop p qh -> in_loop qh qh'.
+    in_loop p qh /\ forall qh', in_loop p qh' -> in_loop qh qh'.
   
   Lemma tag_eq_ex_innermost_lh q q' j l p i :
     TPath' ((q',j) :<: nl_rcons l (q,j))
